LeanPy/Data/VoidRef.lean
@@ -1,0 +1,16 @@
+/-
+Copyright (c) 2025 Mac Malone. All rights reserved.
+Released under the Apache 2.0 license as described in the file LICENSE.
+syntax Authors Mac Malone
+-/
+import LeanPy.Data.MutableRef
+
+namespace LeanPy
+
+/-- A fixed runtime address containing no data. -/
+def VoidRef := MutableRef Unit
+
+deriving instance TypeName for VoidRef
+
+@[inline] def mkVoidRef : BaseIO VoidRef := do
+  mkMutableRef ()
