tests/api.lean
@@ -3,4 +3,4 @@ import LeanPy
 open LeanPy
 
 /-- info: false -/
-#guard_msgs in #eval return (← mkObject).beq (← mkObject)
+#guard_msgs in #eval return (← mkObjectObject).beq (← mkObjectObject)
